[pre-thesis] added BisimulationUptoScript.sml

pre-thesis/UniqueSolutionsScript.sml
@@ -11,6 +11,7 @@ open CCSLib CCSTheory CCSSyntax CCSConv;
 open StrongEQTheory StrongEQLib StrongLawsTheory StrongLawsConv;
 open WeakEQTheory WeakEQLib WeakLawsTheory WeakLawsConv;
 open ObsCongrTheory ObsCongrLib ObsCongrLawsTheory ObsCongrConv;
+open BisimulationUptoTheory;
 open CoarsestCongrTheory;
 
 (* this file contains the theorems of "unique solutions of equations" in CCS *)
@@ -18,139 +19,27 @@ val _ = new_theory "UniqueSolutions";
 
 (******************************************************************************)
 (*                                                                            *)
-(*                     Strong Bisimulation Upto ~                             *)
+(*              CCS expressions and weakly guarded expressions                *)
 (*                                                                            *)
 (******************************************************************************)
-
-(* Define the strong bisimulation relation up to STRONG_EQUIV *)
-val STRONG_BISIM_UPTO = new_definition (
-   "STRONG_BISIM_UPTO",
-  ``STRONG_BISIM_UPTO (Bsm :('a, 'b) simulation) =
-       (!E E'.
-	  Bsm E E' ==>
-	  (!u.
-	   (!E1. TRANS E u E1 ==> 
-		 ?E2. TRANS E' u E2 /\ (STRONG_EQUIV O Bsm O STRONG_EQUIV) E1 E2) /\
-	   (!E2. TRANS E' u E2 ==> 
-		 ?E1. TRANS E u E1 /\ (STRONG_EQUIV O Bsm O STRONG_EQUIV) E1 E2)))``);
-
-val STRONG_BISIM_UPTO_LEMMA = store_thm (
-   "STRONG_BISIM_UPTO_LEMMA",
-  ``!Bsm. STRONG_BISIM_UPTO Bsm ==> STRONG_BISIM (STRONG_EQUIV O Bsm O STRONG_EQUIV)``,
-    GEN_TAC
- >> REWRITE_TAC [STRONG_BISIM, O_DEF]
- >> REPEAT STRIP_TAC (* 2 sub-goals here *)
- >| [ (* goal 1 (of 2) *)
-      Q.PAT_X_ASSUM `STRONG_EQUIV E y'`
-	(STRIP_ASSUME_TAC o (ONCE_REWRITE_RULE [PROPERTY_STAR])) \\
-      POP_ASSUM (STRIP_ASSUME_TAC o (Q.SPEC `u`)) \\
-      POP_ASSUM K_TAC \\
-      RES_TAC \\
-      Q.PAT_X_ASSUM `STRONG_BISIM_UPTO Bsm`
-	(STRIP_ASSUME_TAC o (REWRITE_RULE [STRONG_BISIM_UPTO])) \\
-      RES_TAC \\
-      NTAC 4 (POP_ASSUM K_TAC) \\
-      POP_ASSUM (STRIP_ASSUME_TAC o (REWRITE_RULE [O_DEF])) \\
-      Q.PAT_X_ASSUM `STRONG_EQUIV y E'`
-	(STRIP_ASSUME_TAC o (ONCE_REWRITE_RULE [PROPERTY_STAR])) \\
-      POP_ASSUM (STRIP_ASSUME_TAC o (Q.SPEC `u`)) \\
-      POP_ASSUM K_TAC \\
-      POP_ASSUM (STRIP_ASSUME_TAC o (fn th => MATCH_MP th (ASSUME ``TRANS y u E2'``))) \\
-(***
-   E    ~   y'    Bsm    y    ~   E'
-   |       /              \       |
-   u      u                u      u
-   |     /                  \     |
-   E1 ~ E2 ~ y''' Bsm y'' ~ E2' ~ E2''
- ***)
-      `STRONG_EQUIV E1 y'''` by PROVE_TAC [STRONG_EQUIV_TRANS] \\
-      `STRONG_EQUIV y'' E2''` by PROVE_TAC [STRONG_EQUIV_TRANS] \\
-      Q.EXISTS_TAC `E2''` >> ASM_REWRITE_TAC [] \\
-      Q.EXISTS_TAC `y''` >> ASM_REWRITE_TAC [] \\
-      Q.EXISTS_TAC `y'''` >> ASM_REWRITE_TAC [],
-      (* goal 2 (of 2) *)
-      Q.PAT_X_ASSUM `STRONG_EQUIV y E'`
-	(STRIP_ASSUME_TAC o (ONCE_REWRITE_RULE [PROPERTY_STAR])) \\
-      POP_ASSUM (STRIP_ASSUME_TAC o (Q.SPEC `u`)) \\
-      Q.PAT_X_ASSUM `!E1. TRANS y u E1 ==> P` K_TAC \\
-      RES_TAC \\
-      Q.PAT_X_ASSUM `STRONG_BISIM_UPTO Bsm`
-	(STRIP_ASSUME_TAC o (REWRITE_RULE [STRONG_BISIM_UPTO])) \\
-      RES_TAC \\
-      NTAC 2 (POP_ASSUM K_TAC) \\
-      POP_ASSUM (STRIP_ASSUME_TAC o (REWRITE_RULE [O_DEF])) \\
-      Q.PAT_X_ASSUM `STRONG_EQUIV E y'`
-	(STRIP_ASSUME_TAC o (ONCE_REWRITE_RULE [PROPERTY_STAR])) \\
-      POP_ASSUM (STRIP_ASSUME_TAC o (Q.SPEC `u`)) \\
-      Q.PAT_X_ASSUM `!E1. TRANS E u E1 ==> P` K_TAC \\
-      POP_ASSUM (STRIP_ASSUME_TAC o (fn th => MATCH_MP th (ASSUME ``TRANS y' u E1'``))) \\
-(***
-   E    ~     y'     Bsm    y   ~   E'
-   |         /               \      |
-   u        u                 u     u
-   |       /                   \    |
-   E1'' ~ E1' ~ y''' Bsm y'' ~ E1 ~ E2
- ***)
-      `STRONG_EQUIV E1'' y'''` by PROVE_TAC [STRONG_EQUIV_TRANS] \\
-      `STRONG_EQUIV y'' E2` by PROVE_TAC [STRONG_EQUIV_TRANS] \\
-      Q.EXISTS_TAC `E1''` >> ASM_REWRITE_TAC [] \\
-      Q.EXISTS_TAC `y''` >> ASM_REWRITE_TAC [] \\
-      Q.EXISTS_TAC `y'''` >> ASM_REWRITE_TAC [] ]);
-
-val STRONG_BISIM_SUBSET_EQUIV = store_thm ((* NEW *)
-   "STRONG_BISIM_SUBSET_EQUIV", ``!Bsm. STRONG_BISIM Bsm ==> Bsm RSUBSET STRONG_EQUIV``,
-    PROVE_TAC [RSUBSET, STRONG_EQUIV]);
-
-val STRONG_BISIM_UPTO_EQUIV = store_thm (
-   "STRONG_BISIM_UPTO_EQUIV",
-  ``!Bsm. STRONG_BISIM_UPTO Bsm ==> Bsm RSUBSET STRONG_EQUIV``,
-    REPEAT STRIP_TAC
- >> IMP_RES_TAC STRONG_BISIM_UPTO_LEMMA
- >> IMP_RES_TAC STRONG_BISIM_SUBSET_EQUIV
- >> Suff `Bsm RSUBSET (STRONG_EQUIV O Bsm O STRONG_EQUIV)`
- >- ( DISCH_TAC \\
-      Know `transitive ((RSUBSET) :('a, 'b) simulation -> ('a, 'b) simulation -> bool)`
-      >- PROVE_TAC [RSUBSET_WeakOrder, WeakOrder] \\
-      RW_TAC std_ss [transitive_def] >> RES_TAC )
- >> KILL_TAC
- >> REWRITE_TAC [RSUBSET, O_DEF]
- >> REPEAT STRIP_TAC
- >> `STRONG_EQUIV x x /\ STRONG_EQUIV y y` by PROVE_TAC [STRONG_EQUIV_REFL]
- >> Q.EXISTS_TAC `y` >> ASM_REWRITE_TAC []
- >> Q.EXISTS_TAC `x` >> ASM_REWRITE_TAC []
- (* Hence, to prove P ~ Q, we only have to find a strong bisimulation up to ~
-    which contains (P, Q) *));
-
-(******************************************************************************)
-(*                                                                            *)
-(*                      CCS Equations (X = E[X])                              *)
-(*                                                                            *)
-(******************************************************************************)
-
-(* One-hole context is already defined in CoarsestCongrTheory *)
-val (CONTEXT_rules, CONTEXT_ind, CONTEXT_cases) = Hol_reln `
-    (                     CONTEXT (\x. x)) /\			(* CONTEXT1 *)
-    (!a c.  CONTEXT c ==> CONTEXT (\t. prefix a (c t))) /\	(* CONTEXT2 *)
-    (!x c.  CONTEXT c ==> CONTEXT (\t. sum (c t) x)) /\		(* CONTEXT3 *)
-    (!x c.  CONTEXT c ==> CONTEXT (\t. sum x (c t))) /\		(* CONTEXT4 *)
-    (!x c.  CONTEXT c ==> CONTEXT (\t. par (c t) x)) /\		(* CONTEXT5 *)
-    (!x c.  CONTEXT c ==> CONTEXT (\t. par x (c t))) /\		(* CONTEXT6 *)
-    (!L c.  CONTEXT c ==> CONTEXT (\t. restr L (c t))) /\	(* CONTEXT7 *)
-    (!rf c. CONTEXT c ==> CONTEXT (\t. relab (c t) rf)) `;	(* CONTEXT8 *)
 
 (* Weakly guarded (WG) expressions *)
 val (WG_rules, WG_ind, WG_cases) = Hol_reln `
-    (!a.                         WG (\t. prefix a t)) /\        (* WG1 *)
-    (!p.                         WG (\t. p)) /\                 (* WG2 *)
-    (!a e.   WG e            ==> WG (\t. prefix a (e t))) /\    (* WG3 *)
-    (!e1 e2. WG e1 /\ WG e2  ==> WG (\t. sum (e1 t) (e2 t))) /\ (* WG4 *)
-    (!e1 e2. WG e1 /\ WG e2  ==> WG (\t. par (e1 t) (e2 t))) /\ (* WG5 *)
-    (!L e.   WG e            ==> WG (\t. restr L (e t))) /\     (* WG6 *)
-    (!rf e.  WG e            ==> WG (\t. relab (e t) rf)) `;    (* WG7 *)
+    (!a.                            WG (\t. prefix a t)) /\          (* WG1 *)
+    (!p.                            WG (\t. p)) /\                   (* WG2 *)
+    (!a e.   WG e               ==> WG (\t. prefix a (e t))) /\      (* WG3 *)
+    (!e1 e2. WG e1 /\ WG e2     ==> WG (\t. sum (e1 t) (e2 t))) /\   (* WG4 *)
+    (!e1 e2. WG e1 /\ WG e2     ==> WG (\t. par (e1 t) (e2 t))) /\   (* WG5 *)
+    (!L e.   WG e               ==> WG (\t. restr L (e t))) /\       (* WG6 *)
+    (!rf e.  WG e               ==> WG (\t. relab (e t) rf)) `;      (* WG7 *)
+(*
+    (!X e.   WG e            ==> WG (\t. rec X (e t))) `;            (* WG8 *)
+ *)
 
-val [WG1, WG2, WG3, WG4, WG5, WG6, WG7] =
+val [WG1, WG2, WG3, WG4, WG5, WG6, WG7 (*, WG8 *)] =
     map save_thm
-        (combine (["WG1", "WG2", "WG3", "WG4", "WG5", "WG6", "WG7"], CONJUNCTS WG_rules));
+        (combine (["WG1", "WG2", "WG3", "WG4",
+		   "WG5", "WG6", "WG7" (*, "WG8" *)], CONJUNCTS WG_rules));
 
 (* Expressions = multi-hole (or non-hole) contexts. *)
 val (EXPR_rules, EXPR_ind, EXPR_cases) = Hol_reln `
@@ -161,10 +50,13 @@ val (EXPR_rules, EXPR_ind, EXPR_cases) = Hol_reln `
     (!e1 e2. EXPR e1 /\ EXPR e2 ==> EXPR (\t. par (e1 t) (e2 t))) /\ (* EXPR5 *)
     (!L e.   EXPR e             ==> EXPR (\t. restr L (e t))) /\     (* EXPR6 *)
     (!rf e.  EXPR e             ==> EXPR (\t. relab (e t) rf)) `;    (* EXPR7 *)
+(*
+    (!X e.   EXPR e             ==> EXPR (\t. rec X (e t))) `;       (* EXPR8 *)
+ *)
 
-val [EXPR1, EXPR2, EXPR3, EXPR4, EXPR5, EXPR6, EXPR7] =
+val [EXPR1, EXPR2, EXPR3, EXPR4, EXPR5, EXPR6, EXPR7 (*, EXPR8*)] =
     map save_thm
-        (combine (["EXPR1", "EXPR2", "EXPR3", "EXPR4", "EXPR5", "EXPR6", "EXPR7"],
+        (combine (["EXPR1", "EXPR2", "EXPR3", "EXPR4", "EXPR5", "EXPR6", "EXPR7"(*, "EXPR8"*)],
                   CONJUNCTS EXPR_rules));
 
 val EXPR3a = store_thm ("EXPR3a",
@@ -219,12 +111,12 @@ val WG_IS_EXPR = store_thm (
       MATCH_MP_TAC EXPR4,
       MATCH_MP_TAC EXPR5,
       MATCH_MP_TAC EXPR6,
-      MATCH_MP_TAC EXPR7 ]
+      MATCH_MP_TAC EXPR7 (*, MATCH_MP_TAC EXPR8 *) ]
  >> ASM_REWRITE_TAC []);
 
 (******************************************************************************)
 (*                                                                            *)
-(*                 Unique solutions theorem for ~                             *)
+(*                 Unique solutions theorem for STRONG_EQUIV                  *)
 (*                                                                            *)
 (******************************************************************************)
 
@@ -234,10 +126,11 @@ val WG_IS_EXPR = store_thm (
  *)
 val STRONG_UNIQUE_SOLUTIONS_LEMMA = store_thm (
    "STRONG_UNIQUE_SOLUTIONS_LEMMA",
-  ``!E. WG E ==> !P a P'. TRANS (E P) a P' ==>
+  ``!E. WG E ==>
+	!P a P'. TRANS (E P) a P' ==>
 		 ?E'. EXPR E' /\ (P' = E' P) /\ !Q. TRANS (E Q) a (E' Q)``,
     Induct_on `WG` >> BETA_TAC
- >> COUNT_TAC (rpt STRIP_TAC) (* 7 sub-goals here *)
+ >> COUNT_TAC (rpt STRIP_TAC) (* 8 sub-goals here *)
  >| [ (* goal 1 (of 7) *)
       IMP_RES_TAC TRANS_PREFIX \\
       ASM_REWRITE_TAC [] \\
@@ -536,15 +429,19 @@ val STRONG_UNIQUE_SOLUTIONS = store_thm (
         RW_TAC std_ss [] >| (* 4 sub-goals here *)
         [ (* goal 9.3.1 (of 4) *)
           Q.EXISTS_TAC `y || y''` \\
-          REVERSE CONJ_TAC >- ( MATCH_MP_TAC STRONG_EQUIV_PRESD_BY_PAR >> ASM_REWRITE_TAC [] ) \\
+          REVERSE CONJ_TAC >- ( MATCH_MP_TAC STRONG_EQUIV_PRESD_BY_PAR \\
+				ASM_REWRITE_TAC [] ) \\
           Q.EXISTS_TAC `y || y''` \\
-          CONJ_TAC >- ( MATCH_MP_TAC STRONG_EQUIV_PRESD_BY_PAR >> ASM_REWRITE_TAC [] ) \\
+          CONJ_TAC >- ( MATCH_MP_TAC STRONG_EQUIV_PRESD_BY_PAR \\
+			ASM_REWRITE_TAC [] ) \\
           DISJ1_TAC >> REWRITE_TAC [],
           (* goal 9.3.2 (of 4) *)
           Q.EXISTS_TAC `y || G'' Q` \\
-          REVERSE CONJ_TAC >- ( MATCH_MP_TAC STRONG_EQUIV_PRESD_BY_PAR >> ASM_REWRITE_TAC [] ) \\
+          REVERSE CONJ_TAC >- ( MATCH_MP_TAC STRONG_EQUIV_PRESD_BY_PAR \\
+				ASM_REWRITE_TAC [] ) \\
           Q.EXISTS_TAC `y || G'' P` \\
-          CONJ_TAC >- ( MATCH_MP_TAC STRONG_EQUIV_PRESD_BY_PAR >> ASM_REWRITE_TAC [] ) \\
+          CONJ_TAC >- ( MATCH_MP_TAC STRONG_EQUIV_PRESD_BY_PAR \\
+			ASM_REWRITE_TAC [] ) \\
           DISJ2_TAC \\
           Q.EXISTS_TAC `\t. y || G'' t` >> BETA_TAC >> REWRITE_TAC [] \\
           `EXPR (\z. y)` by REWRITE_TAC [EXPR2] \\
@@ -553,9 +450,11 @@ val STRONG_UNIQUE_SOLUTIONS = store_thm (
           BETA_TAC >> REWRITE_TAC [],
           (* goal 9.3.3 (of 4) *)
           Q.EXISTS_TAC `G'' Q || y''` \\
-          REVERSE CONJ_TAC >- ( MATCH_MP_TAC STRONG_EQUIV_PRESD_BY_PAR >> ASM_REWRITE_TAC [] ) \\
+          REVERSE CONJ_TAC >- ( MATCH_MP_TAC STRONG_EQUIV_PRESD_BY_PAR \\
+				ASM_REWRITE_TAC [] ) \\
           Q.EXISTS_TAC `G'' P || y''` \\
-          CONJ_TAC >- ( MATCH_MP_TAC STRONG_EQUIV_PRESD_BY_PAR >> ASM_REWRITE_TAC [] ) \\
+          CONJ_TAC >- ( MATCH_MP_TAC STRONG_EQUIV_PRESD_BY_PAR \\
+			ASM_REWRITE_TAC [] ) \\
           DISJ2_TAC \\
           Q.EXISTS_TAC `\t. G'' t || y''` >> BETA_TAC >> REWRITE_TAC [] \\
           `EXPR (\z. y'')` by REWRITE_TAC [EXPR2] \\
@@ -564,9 +463,11 @@ val STRONG_UNIQUE_SOLUTIONS = store_thm (
           BETA_TAC >> REWRITE_TAC [],
           (* goal 9.3.4 (of 4) *)
           Q.EXISTS_TAC `G'' Q || G''' Q` \\
-          REVERSE CONJ_TAC >- ( MATCH_MP_TAC STRONG_EQUIV_PRESD_BY_PAR >> ASM_REWRITE_TAC [] ) \\
+          REVERSE CONJ_TAC >- ( MATCH_MP_TAC STRONG_EQUIV_PRESD_BY_PAR \\
+				ASM_REWRITE_TAC [] ) \\
           Q.EXISTS_TAC `G'' P || G''' P` \\
-          CONJ_TAC >- ( MATCH_MP_TAC STRONG_EQUIV_PRESD_BY_PAR >> ASM_REWRITE_TAC [] ) \\
+          CONJ_TAC >- ( MATCH_MP_TAC STRONG_EQUIV_PRESD_BY_PAR \\
+			ASM_REWRITE_TAC [] ) \\
           DISJ2_TAC \\
           Q.EXISTS_TAC `\t. G'' t || G''' t` >> BETA_TAC >> REWRITE_TAC [] \\
           MATCH_MP_TAC EXPR5 >> ASM_REWRITE_TAC [] ] ],
@@ -646,15 +547,19 @@ val STRONG_UNIQUE_SOLUTIONS = store_thm (
         RW_TAC std_ss [] >| (* 4 sub-goals here *)
         [ (* goal 10.3.1 (of 4) *)
           Q.EXISTS_TAC `y'' || y` \\
-          REVERSE CONJ_TAC >- ( MATCH_MP_TAC STRONG_EQUIV_PRESD_BY_PAR >> ASM_REWRITE_TAC [] ) \\
+          REVERSE CONJ_TAC >- ( MATCH_MP_TAC STRONG_EQUIV_PRESD_BY_PAR \\
+				ASM_REWRITE_TAC [] ) \\
           Q.EXISTS_TAC `y'' || y` \\
-          CONJ_TAC >- ( MATCH_MP_TAC STRONG_EQUIV_PRESD_BY_PAR >> ASM_REWRITE_TAC [] ) \\
+          CONJ_TAC >- ( MATCH_MP_TAC STRONG_EQUIV_PRESD_BY_PAR \\
+			ASM_REWRITE_TAC [] ) \\
           DISJ1_TAC >> REWRITE_TAC [],
           (* goal 10.3.2 (of 4) *)
           Q.EXISTS_TAC `G'' Q || y` \\
-          REVERSE CONJ_TAC >- ( MATCH_MP_TAC STRONG_EQUIV_PRESD_BY_PAR >> ASM_REWRITE_TAC [] ) \\
+          REVERSE CONJ_TAC >- ( MATCH_MP_TAC STRONG_EQUIV_PRESD_BY_PAR \\
+				ASM_REWRITE_TAC [] ) \\
           Q.EXISTS_TAC `G'' P || y` \\
-          CONJ_TAC >- ( MATCH_MP_TAC STRONG_EQUIV_PRESD_BY_PAR >> ASM_REWRITE_TAC [] ) \\
+          CONJ_TAC >- ( MATCH_MP_TAC STRONG_EQUIV_PRESD_BY_PAR \\
+			ASM_REWRITE_TAC [] ) \\
           DISJ2_TAC \\
           Q.EXISTS_TAC `\t. G'' t || y` >> BETA_TAC >> REWRITE_TAC [] \\
           `EXPR (\z. y)` by REWRITE_TAC [EXPR2] \\
@@ -663,9 +568,11 @@ val STRONG_UNIQUE_SOLUTIONS = store_thm (
           BETA_TAC >> REWRITE_TAC [],
           (* goal 10.3.3 (of 4) *)
           Q.EXISTS_TAC `y'' || G'' Q` \\
-          REVERSE CONJ_TAC >- ( MATCH_MP_TAC STRONG_EQUIV_PRESD_BY_PAR >> ASM_REWRITE_TAC [] ) \\
+          REVERSE CONJ_TAC >- ( MATCH_MP_TAC STRONG_EQUIV_PRESD_BY_PAR \\
+				ASM_REWRITE_TAC [] ) \\
           Q.EXISTS_TAC `y'' || G'' P` \\
-          CONJ_TAC >- ( MATCH_MP_TAC STRONG_EQUIV_PRESD_BY_PAR >> ASM_REWRITE_TAC [] ) \\
+          CONJ_TAC >- ( MATCH_MP_TAC STRONG_EQUIV_PRESD_BY_PAR \\
+			ASM_REWRITE_TAC [] ) \\
           DISJ2_TAC \\
           Q.EXISTS_TAC `\t. y'' || G'' t` >> BETA_TAC >> REWRITE_TAC [] \\
           `EXPR (\z. y'')` by REWRITE_TAC [EXPR2] \\
@@ -674,7 +581,8 @@ val STRONG_UNIQUE_SOLUTIONS = store_thm (
           BETA_TAC >> REWRITE_TAC [],
           (* goal 10.3.4 (of 4) *)
           Q.EXISTS_TAC `G''' Q || G'' Q` \\
-          REVERSE CONJ_TAC >- ( MATCH_MP_TAC STRONG_EQUIV_PRESD_BY_PAR >> ASM_REWRITE_TAC [] ) \\
+          REVERSE CONJ_TAC >- ( MATCH_MP_TAC STRONG_EQUIV_PRESD_BY_PAR \\
+				ASM_REWRITE_TAC [] ) \\
           Q.EXISTS_TAC `G''' P || G'' P` \\
           CONJ_TAC >- ( MATCH_MP_TAC STRONG_EQUIV_PRESD_BY_PAR >> ASM_REWRITE_TAC [] ) \\
           DISJ2_TAC \\
@@ -691,15 +599,19 @@ val STRONG_UNIQUE_SOLUTIONS = store_thm (
         REWRITE_TAC [O_DEF] >> BETA_TAC >> RW_TAC std_ss [] >| (* 2 sub-goals here *)
         [ (* goal 11.1.1 (of 2) *)
           Q.EXISTS_TAC `restr L y` \\
-          REVERSE CONJ_TAC >- ( MATCH_MP_TAC STRONG_EQUIV_SUBST_RESTR >> ASM_REWRITE_TAC [] ) \\
+          REVERSE CONJ_TAC >- ( MATCH_MP_TAC STRONG_EQUIV_SUBST_RESTR \\
+				ASM_REWRITE_TAC [] ) \\
           Q.EXISTS_TAC `restr L y` \\
-          CONJ_TAC >- ( MATCH_MP_TAC STRONG_EQUIV_SUBST_RESTR >> ASM_REWRITE_TAC [] ) \\
+          CONJ_TAC >- ( MATCH_MP_TAC STRONG_EQUIV_SUBST_RESTR \\
+			ASM_REWRITE_TAC [] ) \\
           DISJ1_TAC >> REWRITE_TAC [],
           (* goal 11.1.2 (of 2) *)
           Q.EXISTS_TAC `restr L (G' Q)` \\
-          REVERSE CONJ_TAC >- ( MATCH_MP_TAC STRONG_EQUIV_SUBST_RESTR >> ASM_REWRITE_TAC [] ) \\
+          REVERSE CONJ_TAC >- ( MATCH_MP_TAC STRONG_EQUIV_SUBST_RESTR \\
+				ASM_REWRITE_TAC [] ) \\
           Q.EXISTS_TAC `restr L (G' P)` \\
-          CONJ_TAC >- ( MATCH_MP_TAC STRONG_EQUIV_SUBST_RESTR >> ASM_REWRITE_TAC [] ) \\
+          CONJ_TAC >- ( MATCH_MP_TAC STRONG_EQUIV_SUBST_RESTR \\
+			ASM_REWRITE_TAC [] ) \\
           DISJ2_TAC \\
           Q.EXISTS_TAC `\t. restr L (G' t)` >> BETA_TAC >> REWRITE_TAC [] \\
           MATCH_MP_TAC EXPR6 >> ASM_REWRITE_TAC [] ],
@@ -711,15 +623,19 @@ val STRONG_UNIQUE_SOLUTIONS = store_thm (
         REWRITE_TAC [O_DEF] >> BETA_TAC >> RW_TAC std_ss [] >| (* 2 sub-goals here *)
         [ (* goal 11.2.1 (of 2) *)
           Q.EXISTS_TAC `restr L y` \\
-          REVERSE CONJ_TAC >- ( MATCH_MP_TAC STRONG_EQUIV_SUBST_RESTR >> ASM_REWRITE_TAC [] ) \\
+          REVERSE CONJ_TAC >- ( MATCH_MP_TAC STRONG_EQUIV_SUBST_RESTR \\
+				ASM_REWRITE_TAC [] ) \\
           Q.EXISTS_TAC `restr L y` \\
-          CONJ_TAC >- ( MATCH_MP_TAC STRONG_EQUIV_SUBST_RESTR >> ASM_REWRITE_TAC [] ) \\
+          CONJ_TAC >- ( MATCH_MP_TAC STRONG_EQUIV_SUBST_RESTR \\
+			ASM_REWRITE_TAC [] ) \\
           DISJ1_TAC >> REWRITE_TAC [],
           (* goal 11.2.2 (of 2) *)
           Q.EXISTS_TAC `restr L (G' Q)` \\
-          REVERSE CONJ_TAC >- ( MATCH_MP_TAC STRONG_EQUIV_SUBST_RESTR >> ASM_REWRITE_TAC [] ) \\
+          REVERSE CONJ_TAC >- ( MATCH_MP_TAC STRONG_EQUIV_SUBST_RESTR \\
+				ASM_REWRITE_TAC [] ) \\
           Q.EXISTS_TAC `restr L (G' P)` \\
-          CONJ_TAC >- ( MATCH_MP_TAC STRONG_EQUIV_SUBST_RESTR >> ASM_REWRITE_TAC [] ) \\
+          CONJ_TAC >- ( MATCH_MP_TAC STRONG_EQUIV_SUBST_RESTR \\
+			ASM_REWRITE_TAC [] ) \\
           DISJ2_TAC \\
           Q.EXISTS_TAC `\t. restr L (G' t)` >> BETA_TAC >> REWRITE_TAC [] \\
           MATCH_MP_TAC EXPR6 >> ASM_REWRITE_TAC [] ] ],
@@ -733,15 +649,19 @@ val STRONG_UNIQUE_SOLUTIONS = store_thm (
         REWRITE_TAC [O_DEF] >> BETA_TAC >> RW_TAC std_ss [] >| (* 2 sub-goals here *)
         [ (* goal 12.1.1 (of 2) *)
           Q.EXISTS_TAC `restr L y` \\
-          REVERSE CONJ_TAC >- ( MATCH_MP_TAC STRONG_EQUIV_SUBST_RESTR >> ASM_REWRITE_TAC [] ) \\
+          REVERSE CONJ_TAC >- ( MATCH_MP_TAC STRONG_EQUIV_SUBST_RESTR \\
+				ASM_REWRITE_TAC [] ) \\
           Q.EXISTS_TAC `restr L y` \\
-          CONJ_TAC >- ( MATCH_MP_TAC STRONG_EQUIV_SUBST_RESTR >> ASM_REWRITE_TAC [] ) \\
+          CONJ_TAC >- ( MATCH_MP_TAC STRONG_EQUIV_SUBST_RESTR \\
+			ASM_REWRITE_TAC [] ) \\
           DISJ1_TAC >> REWRITE_TAC [],
           (* goal 12.1.2 (of 2) *)
           Q.EXISTS_TAC `restr L (G' Q)` \\
-          REVERSE CONJ_TAC >- ( MATCH_MP_TAC STRONG_EQUIV_SUBST_RESTR >> ASM_REWRITE_TAC [] ) \\
+          REVERSE CONJ_TAC >- ( MATCH_MP_TAC STRONG_EQUIV_SUBST_RESTR \\
+				ASM_REWRITE_TAC [] ) \\
           Q.EXISTS_TAC `restr L (G' P)` \\
-          CONJ_TAC >- ( MATCH_MP_TAC STRONG_EQUIV_SUBST_RESTR >> ASM_REWRITE_TAC [] ) \\
+          CONJ_TAC >- ( MATCH_MP_TAC STRONG_EQUIV_SUBST_RESTR \\
+			ASM_REWRITE_TAC [] ) \\
           DISJ2_TAC \\
           Q.EXISTS_TAC `\t. restr L (G' t)` >> BETA_TAC >> REWRITE_TAC [] \\
           MATCH_MP_TAC EXPR6 >> ASM_REWRITE_TAC [] ],
@@ -753,15 +673,19 @@ val STRONG_UNIQUE_SOLUTIONS = store_thm (
         REWRITE_TAC [O_DEF] >> BETA_TAC >> RW_TAC std_ss [] >| (* 2 sub-goals here *)
         [ (* goal 12.2.1 (of 2) *)
           Q.EXISTS_TAC `restr L y` \\
-          REVERSE CONJ_TAC >- ( MATCH_MP_TAC STRONG_EQUIV_SUBST_RESTR >> ASM_REWRITE_TAC [] ) \\
+          REVERSE CONJ_TAC >- ( MATCH_MP_TAC STRONG_EQUIV_SUBST_RESTR \\
+				ASM_REWRITE_TAC [] ) \\
           Q.EXISTS_TAC `restr L y` \\
-          CONJ_TAC >- ( MATCH_MP_TAC STRONG_EQUIV_SUBST_RESTR >> ASM_REWRITE_TAC [] ) \\
+          CONJ_TAC >- ( MATCH_MP_TAC STRONG_EQUIV_SUBST_RESTR \\
+			ASM_REWRITE_TAC [] ) \\
           DISJ1_TAC >> REWRITE_TAC [],
           (* goal 12.2.2 (of 2) *)
           Q.EXISTS_TAC `restr L (G' Q)` \\
-          REVERSE CONJ_TAC >- ( MATCH_MP_TAC STRONG_EQUIV_SUBST_RESTR >> ASM_REWRITE_TAC [] ) \\
+          REVERSE CONJ_TAC >- ( MATCH_MP_TAC STRONG_EQUIV_SUBST_RESTR \\
+				ASM_REWRITE_TAC [] ) \\
           Q.EXISTS_TAC `restr L (G' P)` \\
-          CONJ_TAC >- ( MATCH_MP_TAC STRONG_EQUIV_SUBST_RESTR >> ASM_REWRITE_TAC [] ) \\
+          CONJ_TAC >- ( MATCH_MP_TAC STRONG_EQUIV_SUBST_RESTR \\
+			ASM_REWRITE_TAC [] ) \\
           DISJ2_TAC \\
           Q.EXISTS_TAC `\t. restr L (G' t)` >> BETA_TAC >> REWRITE_TAC [] \\
           MATCH_MP_TAC EXPR6 >> ASM_REWRITE_TAC [] ] ],
@@ -776,13 +700,15 @@ val STRONG_UNIQUE_SOLUTIONS = store_thm (
       REWRITE_TAC [O_DEF] >> BETA_TAC >> RW_TAC std_ss [] >| (* 2 sub-goals here *)
       [ (* goal 13.1 (of 2) *)
         Q.EXISTS_TAC `relab y rf` \\
-        REVERSE CONJ_TAC >- ( MATCH_MP_TAC STRONG_EQUIV_SUBST_RELAB >> ASM_REWRITE_TAC [] ) \\
+        REVERSE CONJ_TAC >- ( MATCH_MP_TAC STRONG_EQUIV_SUBST_RELAB \\
+			      ASM_REWRITE_TAC [] ) \\
         Q.EXISTS_TAC `relab y rf` \\
         CONJ_TAC >- ( MATCH_MP_TAC STRONG_EQUIV_SUBST_RELAB >> ASM_REWRITE_TAC [] ) \\
         DISJ1_TAC >> REWRITE_TAC [],
         (* goal 13.2 (of 2) *)
         Q.EXISTS_TAC `relab (G' Q) rf` \\
-        REVERSE CONJ_TAC >- ( MATCH_MP_TAC STRONG_EQUIV_SUBST_RELAB >> ASM_REWRITE_TAC [] ) \\
+        REVERSE CONJ_TAC >- ( MATCH_MP_TAC STRONG_EQUIV_SUBST_RELAB \\
+			      ASM_REWRITE_TAC [] ) \\
         Q.EXISTS_TAC `relab (G' P) rf` \\
         CONJ_TAC >- ( MATCH_MP_TAC STRONG_EQUIV_SUBST_RELAB >> ASM_REWRITE_TAC [] ) \\
         DISJ2_TAC \\
@@ -798,26 +724,33 @@ val STRONG_UNIQUE_SOLUTIONS = store_thm (
       REWRITE_TAC [O_DEF] >> BETA_TAC >> RW_TAC std_ss [] >| (* 2 sub-goals here *)
       [ (* goal 14.1 (of 2) *)
         Q.EXISTS_TAC `relab y rf` \\
-        REVERSE CONJ_TAC >- ( MATCH_MP_TAC STRONG_EQUIV_SUBST_RELAB >> ASM_REWRITE_TAC [] ) \\
+        REVERSE CONJ_TAC >- ( MATCH_MP_TAC STRONG_EQUIV_SUBST_RELAB \\
+			      ASM_REWRITE_TAC [] ) \\
         Q.EXISTS_TAC `relab y rf` \\
         CONJ_TAC >- ( MATCH_MP_TAC STRONG_EQUIV_SUBST_RELAB >> ASM_REWRITE_TAC [] ) \\
         DISJ1_TAC >> REWRITE_TAC [],
         (* goal 14.2 (of 2) *)
         Q.EXISTS_TAC `relab (G' Q) rf` \\
-        REVERSE CONJ_TAC >- ( MATCH_MP_TAC STRONG_EQUIV_SUBST_RELAB >> ASM_REWRITE_TAC [] ) \\
+        REVERSE CONJ_TAC >- ( MATCH_MP_TAC STRONG_EQUIV_SUBST_RELAB \\
+			      ASM_REWRITE_TAC [] ) \\
         Q.EXISTS_TAC `relab (G' P) rf` \\
         CONJ_TAC >- ( MATCH_MP_TAC STRONG_EQUIV_SUBST_RELAB >> ASM_REWRITE_TAC [] ) \\
         DISJ2_TAC \\
         Q.EXISTS_TAC `\t. relab (G' t) rf` >> BETA_TAC >> REWRITE_TAC [] \\
         MATCH_MP_TAC EXPR7 >> ASM_REWRITE_TAC [] ] ]);
 
-(** Bibliography:
+(* Bibliography:
  *
- * Milner, R.: Communication and concurrency. (1989).
- * Sangiorgi, D.: Equations, contractions, and unique solutions. ACM SIGPLAN Notices. (2015).
+ * [1] Milner, R.: Communication and concurrency. (1989).
+.* [2] Gorrieri, R., Versari, C.: Introduction to Concurrency Theory. Springer, Cham (2015).
+ * [3] Sangiorgi, D.: Introduction to Bisimulation and Coinduction. Cambridge University Press (2011).
+ * [4] Sangiorgi, D., Rutten, J.: Advanced Topics in Bisimulation and Coinduction.
+				  Cambridge University Press (2011).
+ * [5] Sangiorgi, D.: Equations, contractions, and unique solutions. ACM SIGPLAN Notices. (2015).
  *)
 
 val _ = export_theory ();
+val _ = print_theory_to_file "-" "UniqueSolutions.lst";
 val _ = DB.html_theory "UniqueSolutions";
 
 (* last updated: Aug 3, 2017 *)
