pre-thesis/BisimulationUptoScript.sml
@@ -1,0 +1,543 @@
+(*
+ * Copyright 2016-2017  University of Bologna   (Author: Chun Tian)
+ *)
+
+open HolKernel Parse boolLib bossLib;
+
+open pred_setTheory relationTheory pairTheory sumTheory listTheory;
+open prim_recTheory arithmeticTheory combinTheory;
+
+open CCSLib CCSTheory CCSSyntax CCSConv;
+open StrongEQTheory StrongEQLib StrongLawsTheory StrongLawsConv;
+open WeakEQTheory WeakEQLib WeakLawsTheory WeakLawsConv;
+open ObsCongrTheory ObsCongrLib ObsCongrLawsTheory ObsCongrConv;
+
+val _ = new_theory "BisimulationUpto";
+
+(******************************************************************************)
+(*                                                                            *)
+(*                     Strong Bisimulation Upto ~                             *)
+(*                                                                            *)
+(******************************************************************************)
+
+(* Define the strong bisimulation relation up to STRONG_EQUIV *)
+val STRONG_BISIM_UPTO = new_definition (
+   "STRONG_BISIM_UPTO",
+  ``STRONG_BISIM_UPTO (Bsm :('a, 'b) simulation) =
+       (!E E'.
+	  Bsm E E' ==>
+	  (!u.
+	   (!E1. TRANS E u E1 ==> 
+		 ?E2. TRANS E' u E2 /\ (STRONG_EQUIV O Bsm O STRONG_EQUIV) E1 E2) /\
+	   (!E2. TRANS E' u E2 ==> 
+		 ?E1. TRANS E u E1 /\ (STRONG_EQUIV O Bsm O STRONG_EQUIV) E1 E2)))``);
+
+val CONVERSE_STRONG_BISIM_UPTO_lemma = Q.prove (
+   `!Wbsm E E'. (STRONG_EQUIV O (\x y. Wbsm y x) O STRONG_EQUIV) E E' =
+		(STRONG_EQUIV O Wbsm O STRONG_EQUIV) E' E`,
+    rpt GEN_TAC
+ >> EQ_TAC (* 2 sub-goals here *)
+ >| [ (* goal 1 (of 2) *)
+      REWRITE_TAC [O_DEF] >> BETA_TAC >> rpt STRIP_TAC \\
+      `STRONG_EQUIV y' E` by PROVE_TAC [STRONG_EQUIV_SYM] \\
+      `STRONG_EQUIV E' y` by PROVE_TAC [STRONG_EQUIV_SYM] \\
+      Q.EXISTS_TAC `y'` >> ASM_REWRITE_TAC [] \\
+      Q.EXISTS_TAC `y` >> ASM_REWRITE_TAC [],
+      (* goal 2 (of 2) *)
+      REWRITE_TAC [O_DEF] >> BETA_TAC >> rpt STRIP_TAC \\
+      `STRONG_EQUIV E y` by PROVE_TAC [STRONG_EQUIV_SYM] \\
+      `STRONG_EQUIV y' E'` by PROVE_TAC [STRONG_EQUIV_SYM] \\
+      Q.EXISTS_TAC `y'` >> ASM_REWRITE_TAC [] \\
+      Q.EXISTS_TAC `y` >> ASM_REWRITE_TAC [] ]);
+
+val CONVERSE_STRONG_BISIM_UPTO = store_thm (
+   "CONVERSE_STRONG_BISIM_UPTO",
+  ``!Wbsm. STRONG_BISIM_UPTO Wbsm ==> STRONG_BISIM_UPTO (\x y. Wbsm y x)``,
+    GEN_TAC
+ >> PURE_ONCE_REWRITE_TAC [STRONG_BISIM_UPTO]
+ >> BETA_TAC
+ >> rpt STRIP_TAC
+ >> RES_TAC (* 2 sub-goals here *)
+ >| [ (* goal 1 (of 2) *)
+      Q.EXISTS_TAC `E1'` >> ASM_REWRITE_TAC [] \\
+      REWRITE_TAC [CONVERSE_STRONG_BISIM_UPTO_lemma] \\
+      ASM_REWRITE_TAC [],
+      (* goal 2 (of 2) *)
+      Q.EXISTS_TAC `E2'` >> ASM_REWRITE_TAC [] \\
+      REWRITE_TAC [CONVERSE_STRONG_BISIM_UPTO_lemma] \\
+      ASM_REWRITE_TAC [] ]);
+
+val STRONG_BISIM_UPTO_LEMMA = store_thm (
+   "STRONG_BISIM_UPTO_LEMMA",
+  ``!Bsm. STRONG_BISIM_UPTO Bsm ==> STRONG_BISIM (STRONG_EQUIV O Bsm O STRONG_EQUIV)``,
+    GEN_TAC
+ >> REWRITE_TAC [STRONG_BISIM, O_DEF]
+ >> rpt STRIP_TAC (* 2 sub-goals here *)
+ >| [ (* goal 1 (of 2) *)
+      Q.PAT_X_ASSUM `STRONG_EQUIV E y'`
+	(STRIP_ASSUME_TAC o (ONCE_REWRITE_RULE [PROPERTY_STAR])) \\
+      POP_ASSUM (STRIP_ASSUME_TAC o (Q.SPEC `u`)) \\
+      POP_ASSUM K_TAC \\
+      RES_TAC \\
+      Q.PAT_X_ASSUM `STRONG_BISIM_UPTO Bsm`
+	(STRIP_ASSUME_TAC o (REWRITE_RULE [STRONG_BISIM_UPTO])) \\
+      RES_TAC \\
+      NTAC 4 (POP_ASSUM K_TAC) \\
+      POP_ASSUM (STRIP_ASSUME_TAC o (REWRITE_RULE [O_DEF])) \\
+      Q.PAT_X_ASSUM `STRONG_EQUIV y E'`
+	(STRIP_ASSUME_TAC o (ONCE_REWRITE_RULE [PROPERTY_STAR])) \\
+      POP_ASSUM (STRIP_ASSUME_TAC o (Q.SPEC `u`)) \\
+      POP_ASSUM K_TAC \\
+      POP_ASSUM (STRIP_ASSUME_TAC o
+		 (fn th => MATCH_MP th (ASSUME ``TRANS y u E2'``))) \\
+(***
+                  E    ~   y'    Bsm    y    ~   E'
+                  |       /              \       |
+                  u      u                u      u
+                  |     /                  \     |
+                  E1 ~ E2 ~ y''' Bsm y'' ~ E2' ~ E2''
+ ***)
+      `STRONG_EQUIV E1 y'''` by PROVE_TAC [STRONG_EQUIV_TRANS] \\
+      `STRONG_EQUIV y'' E2''` by PROVE_TAC [STRONG_EQUIV_TRANS] \\
+      Q.EXISTS_TAC `E2''` >> ASM_REWRITE_TAC [] \\
+      Q.EXISTS_TAC `y''` >> ASM_REWRITE_TAC [] \\
+      Q.EXISTS_TAC `y'''` >> ASM_REWRITE_TAC [],
+      (* goal 2 (of 2) *)
+      Q.PAT_X_ASSUM `STRONG_EQUIV y E'`
+	(STRIP_ASSUME_TAC o (ONCE_REWRITE_RULE [PROPERTY_STAR])) \\
+      POP_ASSUM (STRIP_ASSUME_TAC o (Q.SPEC `u`)) \\
+      Q.PAT_X_ASSUM `!E1. TRANS y u E1 ==> P` K_TAC \\
+      RES_TAC \\
+      Q.PAT_X_ASSUM `STRONG_BISIM_UPTO Bsm`
+	(STRIP_ASSUME_TAC o (REWRITE_RULE [STRONG_BISIM_UPTO])) \\
+      RES_TAC \\
+      NTAC 2 (POP_ASSUM K_TAC) \\
+      POP_ASSUM (STRIP_ASSUME_TAC o (REWRITE_RULE [O_DEF])) \\
+      Q.PAT_X_ASSUM `STRONG_EQUIV E y'`
+	(STRIP_ASSUME_TAC o (ONCE_REWRITE_RULE [PROPERTY_STAR])) \\
+      POP_ASSUM (STRIP_ASSUME_TAC o (Q.SPEC `u`)) \\
+      Q.PAT_X_ASSUM `!E1. TRANS E u E1 ==> P` K_TAC \\
+      POP_ASSUM (STRIP_ASSUME_TAC o
+		 (fn th => MATCH_MP th (ASSUME ``TRANS y' u E1'``))) \\
+(***
+               E    ~     y'     Bsm    y   ~   E'
+               |         /               \      |
+               u        u                 u     u
+               |       /                   \    |
+               E1'' ~ E1' ~ y''' Bsm y'' ~ E1 ~ E2
+ ***)
+      `STRONG_EQUIV E1'' y'''` by PROVE_TAC [STRONG_EQUIV_TRANS] \\
+      `STRONG_EQUIV y'' E2` by PROVE_TAC [STRONG_EQUIV_TRANS] \\
+      Q.EXISTS_TAC `E1''` >> ASM_REWRITE_TAC [] \\
+      Q.EXISTS_TAC `y''` >> ASM_REWRITE_TAC [] \\
+      Q.EXISTS_TAC `y'''` >> ASM_REWRITE_TAC [] ]);
+
+val STRONG_BISIM_UPTO_EQUIV = store_thm (
+   "STRONG_BISIM_UPTO_EQUIV",
+  ``!Bsm. STRONG_BISIM_UPTO Bsm ==> Bsm RSUBSET STRONG_EQUIV``,
+    rpt STRIP_TAC
+ >> IMP_RES_TAC STRONG_BISIM_UPTO_LEMMA
+ >> IMP_RES_TAC STRONG_BISIM_SUBSET_EQUIV
+ >> Suff `Bsm RSUBSET (STRONG_EQUIV O Bsm O STRONG_EQUIV)`
+ >- ( DISCH_TAC \\
+      Know `transitive ((RSUBSET) :('a, 'b) simulation -> ('a, 'b) simulation -> bool)`
+      >- PROVE_TAC [RSUBSET_WeakOrder, WeakOrder] \\
+      RW_TAC std_ss [transitive_def] >> RES_TAC )
+ >> KILL_TAC
+ >> REWRITE_TAC [RSUBSET, O_DEF]
+ >> rpt STRIP_TAC
+ >> `STRONG_EQUIV x x /\ STRONG_EQUIV y y` by PROVE_TAC [STRONG_EQUIV_REFL]
+ >> Q.EXISTS_TAC `y` >> ASM_REWRITE_TAC []
+ >> Q.EXISTS_TAC `x` >> ASM_REWRITE_TAC []
+ (* Hence, to prove P ~ Q, we only have to find a strong bisimulation up to ~
+    which contains (P, Q) *));
+
+(******************************************************************************)
+(*                                                                            *)
+(*                       Weak Bisimulation Upto ~                             *)
+(*                                                                            *)
+(******************************************************************************)
+
+(* NOTE: the definition in Milner's book [1] is wrong, we use the one in Gorrieri's book [2],
+         double-confirmed with Sangiorgi's book [3].
+
+   IMPORTANT: in HOL's big "O", the second argument to composition acts on the "input" first,
+         so we need to revert the order of (?a O Wbsm O ?b) when ?a and ?b are different.
+ *)
+val WEAK_BISIM_UPTO = new_definition (
+   "WEAK_BISIM_UPTO",
+  ``WEAK_BISIM_UPTO (Wbsm: ('a, 'b) simulation) =
+    !E E'.
+       Wbsm E E' ==>
+       (!l.
+	 (!E1. TRANS E  (label l) E1 ==>
+	       ?E2. WEAK_TRANS E' (label l) E2 /\ (WEAK_EQUIV O Wbsm O STRONG_EQUIV) E1 E2) /\
+	 (!E2. TRANS E' (label l) E2 ==>
+	       ?E1. WEAK_TRANS E  (label l) E1 /\ (STRONG_EQUIV O Wbsm O WEAK_EQUIV) E1 E2)) /\
+       (!E1. TRANS E  tau E1 ==> ?E2. EPS E' E2 /\ (WEAK_EQUIV O Wbsm O STRONG_EQUIV) E1 E2) /\
+       (!E2. TRANS E' tau E2 ==> ?E1. EPS E  E1 /\ (STRONG_EQUIV O Wbsm O WEAK_EQUIV) E1 E2)``);
+
+val WEAK_BISIM_UPTO_TRANS_label = store_thm (
+   "WEAK_BISIM_UPTO_TRANS_label",
+  ``!Wbsm. WEAK_BISIM_UPTO Wbsm ==>
+	!E E'. Wbsm E E' ==>
+	       !l E1. TRANS E (label l) E1 ==>
+		      ?E2. WEAK_TRANS E' (label l) E2 /\ (WEAK_EQUIV O Wbsm O STRONG_EQUIV) E1 E2``,
+    PROVE_TAC [WEAK_BISIM_UPTO]);
+
+val WEAK_BISIM_UPTO_TRANS_label' = store_thm (
+   "WEAK_BISIM_UPTO_TRANS_label'",
+  ``!Wbsm. WEAK_BISIM_UPTO Wbsm ==>
+	!E E'. Wbsm E E' ==>
+	       !l E2. TRANS E' (label l) E2 ==>
+		      ?E1. WEAK_TRANS E  (label l) E1 /\ (STRONG_EQUIV O Wbsm O WEAK_EQUIV) E1 E2``,
+    PROVE_TAC [WEAK_BISIM_UPTO]);
+
+val WEAK_BISIM_UPTO_TRANS_tau = store_thm (
+   "WEAK_BISIM_UPTO_TRANS_tau",
+  ``!Wbsm. WEAK_BISIM_UPTO Wbsm ==>
+	!E E'. Wbsm E E' ==>
+	       !E1. TRANS E tau E1 ==> ?E2. EPS E' E2 /\ (WEAK_EQUIV O Wbsm O STRONG_EQUIV) E1 E2``,
+    PROVE_TAC [WEAK_BISIM_UPTO]);
+
+val WEAK_BISIM_UPTO_TRANS_tau' = store_thm (
+   "WEAK_BISIM_UPTO_TRANS_tau'",
+  ``!Wbsm. WEAK_BISIM_UPTO Wbsm ==>
+	!E E'. Wbsm E E' ==>
+	       !E2. TRANS E' tau E2 ==> ?E1. EPS E  E1 /\ (STRONG_EQUIV O Wbsm O WEAK_EQUIV) E1 E2``,
+    PROVE_TAC [WEAK_BISIM_UPTO]);
+
+val CONVERSE_WEAK_BISIM_UPTO_lemma = Q.prove (
+   `!Wbsm E E'. (WEAK_EQUIV O (\x y. Wbsm y x) O STRONG_EQUIV) E E' =
+		(STRONG_EQUIV O Wbsm O WEAK_EQUIV) E' E`,
+    rpt GEN_TAC
+ >> EQ_TAC (* 2 sub-goals here *)
+ >| [ (* goal 1 (of 2) *)
+      REWRITE_TAC [O_DEF] >> BETA_TAC >> rpt STRIP_TAC \\
+      `STRONG_EQUIV y' E` by PROVE_TAC [STRONG_EQUIV_SYM] \\
+      `WEAK_EQUIV E' y` by PROVE_TAC [WEAK_EQUIV_SYM] \\
+      Q.EXISTS_TAC `y'` >> ASM_REWRITE_TAC [] \\
+      Q.EXISTS_TAC `y` >> ASM_REWRITE_TAC [],
+      (* goal 2 (of 2) *)
+      REWRITE_TAC [O_DEF] >> BETA_TAC >> rpt STRIP_TAC \\
+      `STRONG_EQUIV E y` by PROVE_TAC [STRONG_EQUIV_SYM] \\
+      `WEAK_EQUIV y' E'` by PROVE_TAC [WEAK_EQUIV_SYM] \\
+      Q.EXISTS_TAC `y'` >> ASM_REWRITE_TAC [] \\
+      Q.EXISTS_TAC `y` >> ASM_REWRITE_TAC [] ]);
+
+val CONVERSE_WEAK_BISIM_UPTO_lemma' = Q.prove (
+   `!Wbsm E E'. (STRONG_EQUIV O (\x y. Wbsm y x) O WEAK_EQUIV) E E' =
+		(WEAK_EQUIV O Wbsm O STRONG_EQUIV) E' E`,
+    rpt GEN_TAC
+ >> EQ_TAC (* 2 sub-goals here *)
+ >| [ (* goal 1 (of 2) *)
+      REWRITE_TAC [O_DEF] >> BETA_TAC >> rpt STRIP_TAC \\
+      `STRONG_EQUIV E' y` by PROVE_TAC [STRONG_EQUIV_SYM] \\
+      `WEAK_EQUIV y' E` by PROVE_TAC [WEAK_EQUIV_SYM] \\
+      Q.EXISTS_TAC `y'` >> ASM_REWRITE_TAC [] \\
+      Q.EXISTS_TAC `y` >> ASM_REWRITE_TAC [],
+      (* goal 2 (of 2) *)
+      REWRITE_TAC [O_DEF] >> BETA_TAC >> rpt STRIP_TAC \\
+      `STRONG_EQUIV y' E'` by PROVE_TAC [STRONG_EQUIV_SYM] \\
+      `WEAK_EQUIV E y` by PROVE_TAC [WEAK_EQUIV_SYM] \\
+      Q.EXISTS_TAC `y'` >> ASM_REWRITE_TAC [] \\
+      Q.EXISTS_TAC `y` >> ASM_REWRITE_TAC [] ]);
+
+val CONVERSE_WEAK_BISIM_UPTO = store_thm (
+   "CONVERSE_WEAK_BISIM_UPTO",
+  ``!Wbsm. WEAK_BISIM_UPTO Wbsm ==> WEAK_BISIM_UPTO (\x y. Wbsm y x)``,
+    GEN_TAC
+ >> PURE_ONCE_REWRITE_TAC [WEAK_BISIM_UPTO]
+ >> BETA_TAC
+ >> rpt STRIP_TAC
+ >> RES_TAC (* 4 sub-goals here *)
+ >| [ (* goal 1 (of 4) *)
+      Q.EXISTS_TAC `E1'` >> ASM_REWRITE_TAC [] \\
+      REWRITE_TAC [CONVERSE_WEAK_BISIM_UPTO_lemma] \\
+      ASM_REWRITE_TAC [],
+      (* goal 2 (of 4) *)
+      Q.EXISTS_TAC `E2'` >> ASM_REWRITE_TAC [] \\
+      REWRITE_TAC [CONVERSE_WEAK_BISIM_UPTO_lemma'] \\
+      ASM_REWRITE_TAC [],
+      (* goal 3 (of 4) *)
+      Q.EXISTS_TAC `E1'` >> ASM_REWRITE_TAC [] \\
+      REWRITE_TAC [CONVERSE_WEAK_BISIM_UPTO_lemma] \\
+      ASM_REWRITE_TAC [],
+      (* goal 4 (of 4) *)
+      Q.EXISTS_TAC `E2'` >> ASM_REWRITE_TAC [] \\
+      REWRITE_TAC [CONVERSE_WEAK_BISIM_UPTO_lemma'] \\
+      ASM_REWRITE_TAC [] ]);
+
+val WEAK_BISIM_UPTO_EPS = store_thm ((* NEW *)
+   "WEAK_BISIM_UPTO_EPS",
+  ``!Wbsm. WEAK_BISIM_UPTO Wbsm ==>
+	!E E'. Wbsm E E' ==>
+	       !E1. EPS E E1 ==> ?E2. EPS E' E2 /\ (WEAK_EQUIV O Wbsm O STRONG_EQUIV) E1 E2``,
+    rpt STRIP_TAC
+ >> PAT_X_ASSUM ``WEAK_BISIM_UPTO Wbsm`` MP_TAC
+ >> Q.PAT_X_ASSUM `Wbsm E E'` MP_TAC
+ >> POP_ASSUM MP_TAC
+ >> Q.SPEC_TAC (`E1`, `E1`)
+ >> Q.SPEC_TAC (`E`, `E`)
+ >> HO_MATCH_MP_TAC EPS_ind_right (* must use right induct here! *)
+ >> rpt STRIP_TAC (* 2 sub-goals here *)
+ >| [ (* goal 1 (of 2) *)
+      Q.EXISTS_TAC `E'` \\
+      RW_TAC std_ss [EPS_REFL] \\
+      REWRITE_TAC [O_DEF] >> BETA_TAC \\
+      Q.EXISTS_TAC `E'` >> REWRITE_TAC [WEAK_EQUIV_REFL] \\
+      Q.EXISTS_TAC `E` >> ASM_REWRITE_TAC [STRONG_EQUIV_REFL],
+      (* goal 2 (of 2) *)
+      RES_TAC \\
+      POP_ASSUM (STRIP_ASSUME_TAC o (REWRITE_RULE [O_DEF])) \\
+      STRIP_ASSUME_TAC (ONCE_REWRITE_RULE [PROPERTY_STAR]
+					  (ASSUME ``STRONG_EQUIV E1 y'``)) \\
+      RES_TAC \\
+      NTAC 2 (POP_ASSUM K_TAC) \\
+      STRIP_ASSUME_TAC (REWRITE_RULE [WEAK_BISIM_UPTO]
+				     (ASSUME ``WEAK_BISIM_UPTO Wbsm``)) \\
+      POP_ASSUM (STRIP_ASSUME_TAC o (Q.SPECL [`y'`, `y`])) \\
+      RES_TAC \\
+      NTAC 7 (POP_ASSUM K_TAC) \\
+      Q.PAT_X_ASSUM `Wbsm y' y ==> X` K_TAC \\
+      Q.PAT_X_ASSUM `!l E1. TRANS y' (label l) E1 ==> P` K_TAC \\
+      Q.PAT_X_ASSUM `!l E2. TRANS y (label l) E2 ==> P` K_TAC \\
+      IMP_RES_TAC WEAK_EQUIV_EPS \\
+      Q.EXISTS_TAC `E2'''` \\
+      CONJ_TAC >- IMP_RES_TAC EPS_TRANS \\
+      Q.PAT_X_ASSUM `X E2' E2''` MP_TAC \\
+      REWRITE_TAC [O_DEF] >> BETA_TAC >> rpt STRIP_TAC \\
+(* Induct case:
+      E                Wbsm                E'
+                                           ||
+      ...                                 eps
+                                           ||
+      E1   ~    y'     Wbsm      y    =~   E2
+      |        /                 \\        ||
+     tau     tau                 eps      eps
+      |      /                     \\      ||
+      E1' ~ E2' ~ y''' Wbsm y'' =~ E2'' =~ E2'''
+ *)
+      `WEAK_EQUIV y'' E2'''` by PROVE_TAC [WEAK_EQUIV_TRANS] \\
+      `STRONG_EQUIV E1' y'''` by PROVE_TAC [STRONG_EQUIV_TRANS] \\
+      Q.EXISTS_TAC `y''` >> ASM_REWRITE_TAC [] \\
+      Q.EXISTS_TAC `y'''` >> ASM_REWRITE_TAC [] ]);
+
+val WEAK_BISIM_UPTO_EPS' = store_thm ((* NEW *)
+   "WEAK_BISIM_UPTO_EPS'",
+  ``!Wbsm. WEAK_BISIM_UPTO Wbsm ==>
+	!E E'. Wbsm E E' ==>
+	       !E2. EPS E' E2 ==> ?E1. EPS E E1 /\ (STRONG_EQUIV O Wbsm O WEAK_EQUIV) E1 E2``,
+    GEN_TAC >> DISCH_TAC
+ >> POP_ASSUM (ASSUME_TAC o (MATCH_MP CONVERSE_WEAK_BISIM_UPTO))
+ >> IMP_RES_TAC WEAK_BISIM_UPTO_EPS
+ >> POP_ASSUM MP_TAC
+ >> BETA_TAC >> rpt STRIP_TAC
+ >> RES_TAC
+ >> Q.EXISTS_TAC `E2'` >> ASM_REWRITE_TAC []
+ >> REWRITE_TAC [GSYM CONVERSE_WEAK_BISIM_UPTO_lemma]
+ >> ASM_REWRITE_TAC []);
+
+(* Proof sketch:
+      E            Wbsm              E'
+      ||                             ||
+      eps                            eps
+      ||                             ||
+      E1' ~ y'     Wbsm     y  =~    E2'    (WEAK_BISIM_UPTO_EPS)
+      |     |               ||       ||
+      |     l               l        ||
+      l     |               ||       l
+      |  ~ E2'' (~ Wbsm =~) E2''' =~ ||
+      E2                             E2'''' (WEAK_BISIM_UPTO_TRANS_label)
+      || ~  y'''   Wbsm     y''   =~ ||
+      eps   ||              ||       eps
+      ||    eps             eps      ||
+      ||    ||              ||       ||
+      E1 ~ E2'5 (~ Wbsm =~) E2'6  =~ E2'7   (WEAK_BISIM_UPTO_EPS)
+ *)
+val WEAK_BISIM_UPTO_WEAK_TRANS_label = store_thm ((* NEW *)
+   "WEAK_BISIM_UPTO_WEAK_TRANS_label",
+  ``!Wbsm. WEAK_BISIM_UPTO Wbsm ==>
+	!E E'. Wbsm E E' ==>
+	       !l E1. WEAK_TRANS E (label l) E1 ==>
+		      ?E2. WEAK_TRANS E' (label l) E2 /\
+			   (WEAK_EQUIV O Wbsm O STRONG_EQUIV) E1 E2``,
+    rpt STRIP_TAC
+ >> IMP_RES_TAC WEAK_TRANS
+ >> IMP_RES_TAC (MATCH_MP WEAK_BISIM_UPTO_EPS (* lemma 1 used here *)
+			  (ASSUME ``WEAK_BISIM_UPTO Wbsm``))
+ >> POP_ASSUM (STRIP_ASSUME_TAC o (REWRITE_RULE [O_DEF]))
+ >> IMP_RES_TAC PROPERTY_STAR_TRANS
+ >> IMP_RES_TAC WEAK_BISIM_UPTO_TRANS_label
+ >> POP_ASSUM K_TAC
+ >> IMP_RES_TAC WEAK_EQUIV_WEAK_TRANS_label
+ >> Know `(WEAK_EQUIV O Wbsm O STRONG_EQUIV) E2 E2''''`
+ >- ( Q.PAT_X_ASSUM `X E2'' E2'''` MP_TAC \\
+      REWRITE_TAC [O_DEF] >> BETA_TAC >> rpt STRIP_TAC \\
+      `STRONG_EQUIV E2 y'''` by PROVE_TAC [STRONG_EQUIV_TRANS] \\
+      `WEAK_EQUIV y'' E2''''` by PROVE_TAC [WEAK_EQUIV_TRANS] \\
+      Q.EXISTS_TAC `y''` >> ASM_REWRITE_TAC [] \\
+      Q.EXISTS_TAC `y'''` >> ASM_REWRITE_TAC [] )
+ >> DISCH_TAC
+ >> POP_ASSUM (STRIP_ASSUME_TAC o (REWRITE_RULE [O_DEF]))
+ >> IMP_RES_TAC (MATCH_MP STRONG_EQUIV_EPS
+			  (ASSUME ``STRONG_EQUIV E2 y'''``))
+ >> IMP_RES_TAC (Q.SPECL [`y'''`, `y''`]
+			 (MATCH_MP WEAK_BISIM_UPTO_EPS (* lemma 1 used here *)
+				   (ASSUME ``WEAK_BISIM_UPTO Wbsm``)))
+ >> NTAC 3 (POP_ASSUM K_TAC)
+ >> IMP_RES_TAC (MATCH_MP WEAK_EQUIV_EPS
+			  (ASSUME ``WEAK_EQUIV y'' E2''''``))
+ >> Know `(WEAK_EQUIV O Wbsm O STRONG_EQUIV) E1 E2'''''''`
+ >- ( Q.PAT_X_ASSUM `X E2''''' E2''''''` MP_TAC \\
+      REWRITE_TAC [O_DEF] >> BETA_TAC >> rpt STRIP_TAC \\
+      `STRONG_EQUIV E1 y'''''` by PROVE_TAC [STRONG_EQUIV_TRANS] \\
+      `WEAK_EQUIV y'''' E2'''''''` by PROVE_TAC [WEAK_EQUIV_TRANS] \\
+      Q.EXISTS_TAC `y''''` >> ASM_REWRITE_TAC [] \\
+      Q.EXISTS_TAC `y'''''` >> ASM_REWRITE_TAC [] )
+ >> DISCH_TAC
+ >> Q.EXISTS_TAC `E2'''''''`
+ >> ASM_REWRITE_TAC []
+ >> MATCH_MP_TAC EPS_AND_WEAK
+ >> take [`E2'`, `E2''''`]
+ >> ASM_REWRITE_TAC []);
+
+val WEAK_BISIM_UPTO_WEAK_TRANS_label' = store_thm ((* NEW *)
+   "WEAK_BISIM_UPTO_WEAK_TRANS_label'",
+  ``!Wbsm. WEAK_BISIM_UPTO Wbsm ==>
+	!E E'. Wbsm E E' ==>
+	       !l E2. WEAK_TRANS E' (label l) E2 ==>
+		      ?E1. WEAK_TRANS E (label l) E1 /\
+			   (STRONG_EQUIV O Wbsm O WEAK_EQUIV) E1 E2``,
+    GEN_TAC >> DISCH_TAC
+ >> POP_ASSUM (ASSUME_TAC o (MATCH_MP CONVERSE_WEAK_BISIM_UPTO))
+ >> IMP_RES_TAC WEAK_BISIM_UPTO_WEAK_TRANS_label
+ >> POP_ASSUM MP_TAC
+ >> BETA_TAC >> rpt STRIP_TAC
+ >> RES_TAC
+ >> Q.EXISTS_TAC `E2'` >> ASM_REWRITE_TAC []
+ >> REWRITE_TAC [GSYM CONVERSE_WEAK_BISIM_UPTO_lemma]
+ >> ASM_REWRITE_TAC []);
+
+(* If S is a bisimulation up to WEAK_EQUIV, then (WEAK_EQUIV O S O WEAK_EQUIV) is
+   a (strong? no, weak!) bisimultion. But first, we prove that both:
+     1. (WEAK_EQUIV O S O STRONG_EQUIV) and
+     2. (STRONG_EQUIV O S O WEAK_EQUIV) are weak bisimulations.
+ *)
+val WEAK_BISIM_UPTO_LEMMA = store_thm (
+   "WEAK_BISIM_UPTO_LEMMA",
+  ``!Wbsm. WEAK_BISIM_UPTO Wbsm ==> WEAK_BISIM (WEAK_EQUIV O Wbsm O WEAK_EQUIV)``,
+    GEN_TAC
+ >> REWRITE_TAC [WEAK_BISIM, O_DEF]
+ >> rpt STRIP_TAC (* 4 sub-goals here *)
+ >| [ (* goal 1 (of 4) *)
+      IMP_RES_TAC (MATCH_MP WEAK_EQUIV_TRANS_label (ASSUME ``WEAK_EQUIV E y'``)) \\
+      IMP_RES_TAC (MATCH_MP WEAK_BISIM_UPTO_WEAK_TRANS_label
+			    (ASSUME ``WEAK_BISIM_UPTO Wbsm``)) \\
+      IMP_RES_TAC (MATCH_MP WEAK_EQUIV_WEAK_TRANS_label
+			    (ASSUME ``WEAK_EQUIV y E'``)) \\
+      Q.EXISTS_TAC `E2''` >> ASM_REWRITE_TAC [] \\
+      Q.PAT_X_ASSUM `X E2 E2'` (STRIP_ASSUME_TAC o (REWRITE_RULE [O_DEF])) \\
+(***
+               E    ~=   y'    Wbsm     y    ~=   E'
+               |        //              \\        ||
+              !l       l                 l        l
+               |      //                  \\      ||
+               E1 ~= E2 ~ y''' Wbsm y'' ~= E2' ~= E2''
+ ***)
+      `WEAK_EQUIV E2 y'''` by PROVE_TAC [STRONG_IMP_WEAK_EQUIV] \\
+      `WEAK_EQUIV E1 y'''` by PROVE_TAC [WEAK_EQUIV_TRANS] \\
+      `WEAK_EQUIV y'' E2''` by PROVE_TAC [WEAK_EQUIV_TRANS] \\
+      Q.EXISTS_TAC `y''` >> ASM_REWRITE_TAC [] \\
+      Q.EXISTS_TAC `y'''` >> ASM_REWRITE_TAC [],
+      (* goal 2 (of 4) *)
+      IMP_RES_TAC (MATCH_MP WEAK_EQUIV_TRANS_label' (ASSUME ``WEAK_EQUIV y E'``)) \\
+      IMP_RES_TAC (MATCH_MP WEAK_BISIM_UPTO_WEAK_TRANS_label'
+			    (ASSUME ``WEAK_BISIM_UPTO Wbsm``)) \\
+      IMP_RES_TAC (MATCH_MP WEAK_EQUIV_WEAK_TRANS_label'
+			    (ASSUME ``WEAK_EQUIV E y'``)) \\
+      Q.EXISTS_TAC `E1''` >> ASM_REWRITE_TAC [] \\
+      Q.PAT_X_ASSUM `X E1' E1` (STRIP_ASSUME_TAC o (REWRITE_RULE [O_DEF])) \\
+(***
+               E    ~=     y'      Wbsm    y   ~=   E'
+               ||         //               \\       |
+               l         l                  l       l
+               ||       //                   \\     |
+               E1'' ~= E1' ~= y''' Wbsm y'' ~ E1 ~= E2
+ ***)
+      `WEAK_EQUIV E1'' y'''` by PROVE_TAC [WEAK_EQUIV_TRANS] \\
+      `WEAK_EQUIV y'' E1` by PROVE_TAC [STRONG_IMP_WEAK_EQUIV] \\
+      `WEAK_EQUIV y'' E2` by PROVE_TAC [WEAK_EQUIV_TRANS] \\
+      Q.EXISTS_TAC `y''` >> ASM_REWRITE_TAC [] \\
+      Q.EXISTS_TAC `y'''` >> ASM_REWRITE_TAC [],
+      (* goal 3 (of 4) *)
+      IMP_RES_TAC (MATCH_MP WEAK_EQUIV_TRANS_tau (ASSUME ``WEAK_EQUIV E y'``)) \\
+      IMP_RES_TAC (MATCH_MP WEAK_BISIM_UPTO_EPS (ASSUME ``WEAK_BISIM_UPTO Wbsm``)) \\
+      IMP_RES_TAC (MATCH_MP WEAK_EQUIV_EPS (ASSUME ``WEAK_EQUIV y E'``)) \\
+      Q.EXISTS_TAC `E2''` >> ASM_REWRITE_TAC [] \\
+      Q.PAT_X_ASSUM `X E2 E2'` (STRIP_ASSUME_TAC o (REWRITE_RULE [O_DEF])) \\
+(***
+               E    ~=   y'    Wbsm     y    ~=   E'
+               |        //              \\        ||
+              tau      eps               eps      eps
+               |      //                  \\      ||
+               E1 ~= E2 ~ y''' Wbsm y'' ~= E2' ~= E2''
+ ***)
+      `WEAK_EQUIV E2 y'''` by PROVE_TAC [STRONG_IMP_WEAK_EQUIV] \\
+      `WEAK_EQUIV E1 y'''` by PROVE_TAC [WEAK_EQUIV_TRANS] \\
+      `WEAK_EQUIV y'' E2''` by PROVE_TAC [WEAK_EQUIV_TRANS] \\
+      Q.EXISTS_TAC `y''` >> ASM_REWRITE_TAC [] \\
+      Q.EXISTS_TAC `y'''` >> ASM_REWRITE_TAC [],
+      (* goal 4 (of 4) *)
+      IMP_RES_TAC (MATCH_MP WEAK_EQUIV_TRANS_tau' (ASSUME ``WEAK_EQUIV y E'``)) \\
+      IMP_RES_TAC (MATCH_MP WEAK_BISIM_UPTO_EPS' (ASSUME ``WEAK_BISIM_UPTO Wbsm``)) \\
+      IMP_RES_TAC (MATCH_MP WEAK_EQUIV_EPS' (ASSUME ``WEAK_EQUIV E y'``)) \\
+      Q.EXISTS_TAC `E1''` >> ASM_REWRITE_TAC [] \\
+      Q.PAT_X_ASSUM `X E1' E1` (STRIP_ASSUME_TAC o (REWRITE_RULE [O_DEF])) \\
+(***
+               E    ~=     y'      Wbsm    y   ~=   E'
+               ||         //               \\       |
+               eps       eps                eps     tau
+               ||       //                   \\     |
+               E1'' ~= E1' ~= y''' Wbsm y'' ~ E1 ~= E2
+ ***)
+      `WEAK_EQUIV E1'' y'''` by PROVE_TAC [WEAK_EQUIV_TRANS] \\
+      `WEAK_EQUIV y'' E1` by PROVE_TAC [STRONG_IMP_WEAK_EQUIV] \\
+      `WEAK_EQUIV y'' E2` by PROVE_TAC [WEAK_EQUIV_TRANS] \\
+      Q.EXISTS_TAC `y''` >> ASM_REWRITE_TAC [] \\
+      Q.EXISTS_TAC `y'''` >> ASM_REWRITE_TAC [] ]);
+
+val WEAK_BISIM_UPTO_EQUIV = store_thm (
+   "WEAK_BISIM_UPTO_EQUIV",
+  ``!Wbsm. WEAK_BISIM_UPTO Wbsm ==> Wbsm RSUBSET WEAK_EQUIV``,
+    rpt STRIP_TAC
+ >> IMP_RES_TAC WEAK_BISIM_UPTO_LEMMA
+ >> IMP_RES_TAC WEAK_BISIM_SUBSET_EQUIV
+ >> Suff `Wbsm RSUBSET (WEAK_EQUIV O Wbsm O WEAK_EQUIV)`
+ >- ( DISCH_TAC \\
+      Know `transitive ((RSUBSET) :('a, 'b) simulation -> ('a, 'b) simulation -> bool)`
+      >- PROVE_TAC [RSUBSET_WeakOrder, WeakOrder] \\
+      RW_TAC std_ss [transitive_def] >> RES_TAC )
+ >> KILL_TAC
+ >> REWRITE_TAC [RSUBSET, O_DEF]
+ >> rpt STRIP_TAC
+ >> `WEAK_EQUIV x x /\ WEAK_EQUIV y y` by PROVE_TAC [WEAK_EQUIV_REFL]
+ >> Q.EXISTS_TAC `y` >> ASM_REWRITE_TAC []
+ >> Q.EXISTS_TAC `x` >> ASM_REWRITE_TAC []
+ (* Hence, to prove P =~ Q, we only have to find a strong bisimulation up to =~
+    which contains (P, Q) *));
+
+(* Bibliography:
+ *
+ * [1] Milner, R.: Communication and concurrency. (1989).
+.* [2] Gorrieri, R., Versari, C.: Introduction to Concurrency Theory. Springer, Cham (2015).
+ * [3] Sangiorgi, D.: Introduction to Bisimulation and Coinduction. Cambridge University Press (2011).
+ * [4] Sangiorgi, D., Rutten, J.: Advanced Topics in Bisimulation and Coinduction.
+				  Cambridge University Press (2011).
+ *)
+
+val _ = export_theory ();
+val _ = print_theory_to_file "-" "BisimulationUpto.lst";
+val _ = DB.html_theory "BisimulationUpto";
+
+(* last updated: Aug 5, 2017 *)
